R1cs.v
@@ -1,6 +1,7 @@
 Require Import Metalib.Metatheory.
 From STLCZK Require Import GaloisField.
 From STLCZK Require Import Ltac.
+From STLCZK Require Import NonEmpty.
 Require Import Coqprime.elliptic.ZEll.
 Require Import Coq.Numbers.BinNums.
 Require Import Coqprime.elliptic.GZnZ.
@@ -19,204 +20,235 @@ Module R1CS(PF: GaloisField).
   Import PF.
   Import VectorNotations.
   Definition Vfp := Vector.t Fp.
-  
-  Inductive term: nat -> nat -> nat -> Set :=
-  | input: forall (n: nat), term (S n) 0 0
-  | output: forall (n: nat), term 0 (S n) 0
-  | var: forall (n: nat), term 0 0 (S n)
-  | one: term 0 0 0.
 
-  Inductive additions: nat -> nat -> nat -> Type :=
-  | ahead: forall i o v, Fp * term i o v -> additions i o v
-  | atail: forall i o v i' o' v',
-      Fp * term i o v ->
-      additions i' o' v' ->
-      additions (max i i') (max o o') (max v v').
+  Class Computable(A : Type)(R: Type) :=
+    {
+    (** Substitute input i[0] with one, i[S n] -> i[n] *)
+    subst: A -> Fp -> A;
+    
+    (** Get number of free inputs *)
+    num_inputs: A -> nat;
+    
+    (** Get number of free vars *)
+    num_vars: A -> nat;
+    
+    (** Evaluate to a number *)
+    eval{i v}(a: A):
+                     num_inputs a < i ->
+                     num_vars a < v ->
+                     Vfp i ->
+                     Vfp v ->
+                     Fp ->
+                     R
+    }.
   
-  Inductive constraint: nat -> nat -> nat -> Type :=
-  | lc: forall i o v i' o' v' i'' o'' v''
-      (A: additions i o v)
-      (B: additions i' o' v')
-      (C: additions i'' o'' v''),
-      constraint (max i (max i' i'')) (max o (max o' o'')) (max v (max v' v'')).
+  Inductive term: Set :=
+  | input(f: Fp)(n: nat): term
+  | var(f: Fp)(n: nat): term
+  | output(f: Fp): term
+  | one(f: Fp): term.
 
-  Inductive r1cs: nat -> nat -> nat -> nat -> Type :=
-  | rnil: r1cs 0 0 0 0
-  | rcons: forall n i o v i' o' v',
-      constraint i o v ->
-      r1cs n i' o' v' ->
-      r1cs (S n) (max i i') (max o o') (max v v').
 
+  Definition additions :=
+    NonEmpty term.
   
-  Arguments additions {i} {o} {v}.
-  Arguments ahead {i} {o} {v}.
-  Arguments atail {i} {o} {v} {i'} {o'} {v'}.
-  Arguments constraint {i} {o} {v}.
-  Arguments lc {i} {o} {v} {i'} {o'} {v'} {i''} {o''} {v''}.
-  Arguments rcons {n} {i} {o} {v} {i'} {o'} {v'}.
-  Arguments r1cs {n} {i} {o} {v}.
-  
-  Definition r1cs_singleton{i o v}(c: @constraint i o v) :=
-    rcons c rnil.
+  Inductive constraint: Set :=
+  | lc (A: additions) (B: additions) (C: additions).
+
+  Definition r1cs :=
+    NonEmpty constraint.
 
   (** syntax *)
   Declare Custom Entry r1cs.
-  
-  Notation "<[ x ; .. ; y ]>" :=
-    (rcons x .. (rcons y rnil) ..)
-      (at level 1,
-          x custom r1cs at level 2,
-          y custom r1cs at level 2,
-          left associativity).
 
+  Notation "<[ x ]>" :=
+    (@NE_Sing constraint x) (x custom r1cs at level 99).
+
+  Notation "x ++ y" :=
+    (NE_app x y): seq_notations.
+  
   Notation "'{' a '*' b '==' c '}'" :=
     (lc a b c)
-      (in custom r1cs at level 2,
-          a custom r1cs at level 3,
-          b custom r1cs at level 3,
-          c custom r1cs at level 3,
+      (in custom r1cs at level 80,
+          a custom r1cs at level 40,
+          b custom r1cs at level 40,
+          c custom r1cs at level 40,
           left associativity).
 
   Notation "( a )" :=
-    (ahead a) (in custom r1cs at level 3, a custom r1cs at level 4).
+    (NE_Sing a) (in custom r1cs at level 40, a custom r1cs at level 5).
   
   Notation "( a1 + .. + a2 + a3 )" :=
-    (atail a1 .. (atail a2 (ahead a3)) ..)
-      (in custom r1cs at level 3,
-          a1 custom r1cs at level 4,
-          a2 custom r1cs at level 4,
-          a3 custom r1cs at level 4).
+    (NE_Cons a1 .. (NE_Cons a2 (NE_Sing a3)) ..)
+      (in custom r1cs at level 40,
+          a1 custom r1cs at level 5,
+          a2 custom r1cs at level 5,
+          a3 custom r1cs at level 5).
   
   Notation "z 'i[' n ']'" :=
-    (to_p z, input n%nat)
-      (in custom r1cs at level 4,
+    (input (to_p z) n%nat)
+      (in custom r1cs at level 5,
           n constr,
           z constr).
   
-  Notation "z 'o[' n ']'" :=
-    (to_p z, output n%nat)
-      (in custom r1cs at level 4,
-          n constr,
+  Notation "z 'o'" :=
+    (output (to_p z))
+      (in custom r1cs at level 5,
           z constr).
   
   Notation "z 'v[' n ']'" :=
-    (to_p z, var n%nat)
-      (in custom r1cs at level 4,
+    (var (to_p z) n%nat)
+      (in custom r1cs at level 5,
           n constr,
           z constr).
 
   Notation "[ z ]" :=
-    (to_p z, one)
-      (in custom r1cs at level 4,
+    (one (to_p z))
+      (in custom r1cs at level 5,
           z constr at level 0).
 
+  Definition r1cs_singleton(c: constraint): r1cs :=
+    NE_Sing c.
+ 
   Coercion r1cs_singleton: constraint >-> r1cs.
-  Eval cbn in <[ { (3o[0] + 3i[1]) * (3i[0] + 2v[2]) == ([1]) };{ (3o[0] + 3i[1]) * (3i[0] + 2v[2]) == ([1]) }  ]>.   
 
-  Fixpoint eval_additions{i o v i' o' v'}
-           (adds: @additions i o v)
-           (inputs: Vfp i')
-           (outputs: Vfp o')
-           (vars: Vfp v'): i <= i' -> o <= o' -> v <= v' -> Fp.
-    invert adds; intros.
-    - invert H; invert H4.
-      + apply le_lt_Sn_m in H0; clear H1 H2.
-        exact (pkmul H3 (Vector.nth inputs (Fin.of_nat_lt H0))).  (** Fp * Input term *)
-      + apply le_lt_Sn_m in H1; clear H0 H2.
-        exact (pkmul H3 (Vector.nth outputs (Fin.of_nat_lt H1))). (** Fp * Output term *)
-      + apply le_lt_Sn_m in H2; clear H0 H1.
-        exact (pkmul H3 (Vector.nth vars (Fin.of_nat_lt H2))).    (** Fp * Var term *)
-      + exact H3. (** Fp * 1 (One) term *)
-    - specialize (eval_additions _ _ _ _ _ _ H0 inputs outputs vars) as Hprev.
-      pose proof (Nat.max_lub_r _ _ _ H1).
-      pose proof (Nat.max_lub_r _ _ _ H2).
-      pose proof (Nat.max_lub_r _ _ _ H3).
-      pose proof (Nat.max_lub_l _ _ _ H1).
-      pose proof (Nat.max_lub_l _ _ _ H2).
-      pose proof (Nat.max_lub_l _ _ _ H3).
-      clear H1 H2 H3.
-      invert H; invert H2.
-      + apply le_lt_Sn_m in H7; clear H8 H9.
-        exact (pkplus (Hprev H4 H5 H6) (pkmul H1 (Vector.nth inputs (Fin.of_nat_lt H7)))).
-      + apply le_lt_Sn_m in H8; clear H7 H9.
-        exact (pkplus (Hprev H4 H5 H6) (pkmul H1 (Vector.nth outputs (Fin.of_nat_lt H8)))).
-      + apply le_lt_Sn_m in H9; clear H7 H8.
-        exact (pkplus (Hprev H4 H5 H6) (pkmul H1 (Vector.nth vars (Fin.of_nat_lt H9)))).
-      + exact (pkplus (Hprev H4 H5 H6) H1).
+  Local Open Scope seq_notations.
+  (** An example syntax *)
+  Eval cbn in
+      <[ { (3o + 3i[1]) * (3i[0] + 2v[2]) == ([1]) } ]>
+      ++ <[ { (3o + 3i[1]) * (3i[0] + 2v[2]) == ([1]) } ]>.
+ 
+  #[refine] Instance term_Computable: Computable term Fp :=
+    {
+    subst t k :=
+      match t with
+      | input m 0 => one (pkmul m k)
+      | input a (S n) => input a n
+      | _ => t
+      end;
+    num_inputs t :=
+      match t with
+      | input f n => n
+      | _ => 0%nat
+      end;
+    num_vars t :=
+      match t with
+      | var f n => n
+      | _ => 0%nat
+      end;
+    }.
+  intros i v a Hi Hv inps vars out; destruct a eqn:Ha.
+  - exact (pkmul f (Vector.nth inps (Fin.of_nat_lt Hi))).
+  - exact (pkmul f (Vector.nth vars (Fin.of_nat_lt Hv))).
+  - exact (pkmul f out).
+  - exact f.
   Defined.
 
-  Fixpoint eval_constraint{i o v i' o' v'}
-           (ctr: @constraint i o v)
-           (inputs: Vfp i')
-           (outputs: Vfp o')
-           (vars: Vfp v') : i <= i' -> o <= o' -> v <= v' -> Fp.
-    invert ctr.
-    intros.
-    pose proof (Nat.max_lub_r _ _ _ H).
-    pose proof (Nat.max_lub_r _ _ _ H0).
-    pose proof (Nat.max_lub_r _ _ _ H1).
-    pose proof (Nat.max_lub_l _ _ _ H).
-    pose proof (Nat.max_lub_l _ _ _ H0).
-    pose proof (Nat.max_lub_l _ _ _ H1).
-    pose proof (Nat.max_lub_r _ _ _ H2).
-    pose proof (Nat.max_lub_r _ _ _ H3).
-    pose proof (Nat.max_lub_r _ _ _ H4).
-    pose proof (Nat.max_lub_l _ _ _ H2).
-    pose proof (Nat.max_lub_l _ _ _ H3).
-    pose proof (Nat.max_lub_l _ _ _ H4).    
-    clear H H0 H1 H2 H3 H4.
-    pose proof (eval_additions A inputs outputs vars H5 H6 H7) as SumA.
-    pose proof (eval_additions B inputs outputs vars H11 H12 H13) as SumB.
-    pose proof (eval_additions C inputs outputs vars H8 H9 H10) as SumC.
-    exact (pksub (pkmul SumA SumB) SumC). (** A * B - C *)
+  #[refine] Instance additions_Computable: Computable additions Fp :=
+    {
+    subst t k := NE_map (fun x => subst x k) t;
+      
+    num_inputs t :=
+        NE_max (NE_map num_inputs t);
+        
+    num_vars t :=
+        NE_max (NE_map num_vars t); 
+    }.
+  intros i v a; induction a; intros Hi Hv inps vars out.
+  - rewrite NE_map_sing in Hi, Hv.
+    apply NE_max_sing in Hi.
+    apply NE_max_sing in Hv.
+    exact (eval a Hi Hv inps vars out).
+  - rewrite NE_map_cons in Hi, Hv.
+    remember (num_inputs a) as ih.
+    remember (NE_map num_inputs a0) as its.
+    remember (num_vars a) as vh.
+    remember (NE_map num_vars a0) as vts.
+    apply NE_max_cons in Hv; destruct Hv.
+    apply NE_max_cons in Hi; destruct Hi.
+    rewrite Heqvh in H.
+    rewrite Heqih in H1.
+    exact (pkplus
+             (IHa H2 H0 inps vars out)
+             (eval a H1 H inps vars out)).
   Defined.
 
-  Import VectorNotations.
-  Fixpoint eval_fix{n i o v i' o' v'}
-           (r: @r1cs n i o v)
-           (inputs: Vfp i')
-           (outputs: Vfp o')
-           (vars: Vfp v'): i <= i' -> o <= o' -> v <= v' -> Vfp n.
-  Proof.
-    intros.
-    invert r.
-    - exact [].
-    - pose proof (Nat.max_lub_r _ _ _ H).
-      pose proof (Nat.max_lub_l _ _ _ H).
-      pose proof (Nat.max_lub_r _ _ _ H0).
-      pose proof (Nat.max_lub_l _ _ _ H0).
-      pose proof (Nat.max_lub_r _ _ _ H1).
-      pose proof (Nat.max_lub_l _ _ _ H1).      
-      pose proof (eval_fix _ _ _ _ _ _ _ H3 inputs outputs vars H4 H6 H8) as Hprev.
-      pose proof (eval_constraint H2 inputs outputs vars H5 H7 H9) as CtrEval.
-      exact (CtrEval :: Hprev). 
+  #[refine] Instance constraint_Computable: Computable constraint Fp :=
+    {
+    subst t k :=
+      match t with lc a b c => lc (subst a k) (subst b k) (subst c k) end;
+                 
+    num_inputs t :=
+      match t with lc a b c => max (num_inputs a) (max (num_inputs b) (num_inputs c)) end;
+                
+    num_vars t :=
+      match t with lc a b c => max (num_vars a) (max (num_vars b) (num_vars c)) end;
+    }.
+  intros i v a H H0 inps vars out; destruct a eqn:Ha; subst.
+  apply Nat.max_lub_lt_iff in H.
+  destruct H.
+  apply Nat.max_lub_lt_iff in H1.
+  destruct H1.
+  apply Nat.max_lub_lt_iff in H0.
+  destruct H0.
+  apply Nat.max_lub_lt_iff in H3.
+  destruct H3.
+  pose proof (eval A H H0 inps vars out) as RA.
+  pose proof (eval B H1 H3 inps vars out) as RB.
+  pose proof (eval C H2 H4 inps vars out) as RC.
+  exact (pksub (pkmul RA RB) RC).
   Defined.
 
-  Definition eval{n i o v i' o' v'}
-             (r: @r1cs n i o v)(inputs: Vfp i')(outputs: Vfp o')(vars: Vfp v')
-             {Hi: i <= i'} {Ho: o <= o'} {Hv: v <= v'} :=
-    @eval_fix n i o v i' o' v' r inputs outputs vars Hi Ho Hv.
+  #[refine] Instance r1cs_Computable: Computable r1cs Prop :=
+    {
+    subst t k := NE_map (fun x => subst x k) t;
+      
+    num_inputs t :=
+      NE_max (NE_map num_inputs t);
+        
+    num_vars t :=
+        NE_max (NE_map num_vars t); 
+    }.
+  intros i v a; induction a; intros Hi Hv inps vars out.
+  - rewrite NE_map_sing in Hi, Hv.
+    apply NE_max_sing in Hi.
+    apply NE_max_sing in Hv.
+    exact (eval a Hi Hv inps vars out = 0:%p).
+  - rewrite NE_map_cons in Hi, Hv.
+    apply NE_max_cons in Hi.
+    apply NE_max_cons in Hv.
+    destruct Hi.
+    destruct Hv.
+    exact (IHa H0 H2 inps vars out /\ eval a H H1 inps vars out = 0:%p).
+  Defined.
   
-  Definition correct_lt{n i o v i' o' v'}
-             (r: @r1cs n i o v)(inputs: Vfp i')(outputs: Vfp o')(vars: Vfp v')
-             {Hi: i <= i'}{Ho: o <= o'}{Hv: v <= v'}: Prop :=
-    let values := @eval n i o v i' o' v' r inputs outputs vars Hi Ho Hv in
-    Vector.Forall (fun v => v = 0:%p) values.
-
-  Definition correct{n i o v}(r: @r1cs n i o v)(inputs: Vfp i)(outputs: Vfp o)(vars: Vfp v): Prop :=
-    @correct_lt n i o v i o v r inputs outputs vars (Nat.le_refl i)(Nat.le_refl o)(Nat.le_refl v).
+  Definition correct(r: r1cs)
+             (inputs: Vfp (S (num_inputs r)))
+             (output: Fp)
+             (vars: Vfp (S (num_vars r))): Prop :=
+    @eval r1cs Prop r1cs_Computable
+     (S (@num_inputs r1cs Prop r1cs_Computable r))
+     (S (@num_vars r1cs Prop r1cs_Computable r))
+     r
+     (Nat.lt_succ_diag_r (@num_inputs r1cs Prop r1cs_Computable r))
+     (Nat.lt_succ_diag_r (@num_vars r1cs Prop r1cs_Computable r))
+     inputs
+     vars
+     output.
+     
 
   Import VectorNotations.
   Unset Printing Implicit.
   Lemma example_correct1:
-    correct <[ { (1i[0]) * (1i[1]) == (1o[0]) } ]> [1:%p; 1:%p] [1:%p] [].
+    correct <[ { (1i[0]) * (1i[1]) == (1o) } ]> [1:%p; 1:%p] 1:%p [0:%p].
   Proof.
-    unfold correct, correct_lt.
-    cbn.
-    constructor.
+    unfold correct.
+    
+    simpl.
+    Check (Nat.max_lub_lt_iff 0 1 2).
     destruct FTH.
     inversion F_R.
-    - autorewrite with pk using trivial.
+    - cbn. autorewrite with pk using trivial.
     - constructor.
   Qed.
 
